Progress towards first part of type soundness

typing/pure_typingProofScript.sml
@@ -1,9 +1,19 @@
 open HolKernel Parse boolLib bossLib BasicProvers;
 open pairTheory arithmeticTheory integerTheory stringTheory optionTheory
-     listTheory alistTheory;
-open pure_cexpTheory pure_configTheory pure_typingTheory pure_typingPropsTheory
+     listTheory rich_listTheory alistTheory finite_mapTheory;
+open pure_miscTheory pure_configTheory pure_expTheory pure_exp_lemmasTheory
+     pure_evalTheory pure_cexpTheory pure_cexp_lemmasTheory
+     pure_typingTheory pure_typingPropsTheory;
 
 val _ = new_theory "pure_typingProof";
+
+(* TODO replace existing get_atoms_SOME_SOME_eq *)
+Theorem get_atoms_SOME_SOME_eq:
+  ∀ls as. get_atoms ls = SOME (SOME as) ⇔ ls = MAP wh_Atom as
+Proof
+  rw[get_atoms_SOME_SOME_eq] >>
+  rw[LIST_EQ_REWRITE, LIST_REL_EL_EQN] >> eq_tac >> gvs[EL_MAP]
+QED
 
 Theorem eval_op_type_safe:
   (type_atom_op op ts t ∧ t ≠ Bool ∧
@@ -28,6 +38,211 @@ Proof
   >- (IF_CASES_TAC >> gvs[])
 QED
 
+(* TODO: can't have α in α cexp free, so we use unit here.
+   We should prove a basic theorem about types not caring about the α. *)
+Inductive type_wh:
+  (type_cexp ns db st env (Prim () (Cons s) ces) t ∧
+   MAP exp_of ces = es ⇒
+    type_wh ns db st env (wh_Constructor s es) t) ∧
+
+  (type_cexp ns db st env (ce : unit cexp) t ∧
+   exp_of ce = Lam s e ⇒
+    type_wh ns db st env (wh_Closure s e) t) ∧
+
+  (type_cexp ns db st env (Prim () (AtomOp $ Lit l) []) t ⇒
+    type_wh ns db st env (wh_Atom l) t) ∧
+
+  (type_ok (SND ns) db t ⇒ type_wh ns db st env wh_Diverge t)
+End
+
+Triviality type_wh_PrimTy_eq_wh_Atom:
+  type_wh ns db st env wh (PrimTy pt) ∧ pt ≠ Bool ⇒
+    wh = wh_Diverge ∨ ∃a. wh = wh_Atom a
+Proof
+  rw[type_wh_cases]
+  >- gvs[Once type_cexp_cases] >>
+  reverse $ Cases_on `ce` >> gvs[exp_of_def] >>
+  gvs[Once type_cexp_cases] >>
+  Cases_on `l` using SNOC_CASES >> gvs[MAP_SNOC, Apps_SNOC]
+QED
+
+Triviality type_cexp_type_ok_unit =
+  type_cexp_type_ok |> INST_TYPE [alpha |-> ``:unit``];
+
+Theorem type_soundness:
+  ∀k (ce : unit cexp) ns db st t.
+    namespace_ok ns ∧
+    EVERY (type_ok (SND ns) db) st ∧
+    type_cexp ns db st [] ce t
+  ⇒ ∃wh. eval_wh_to k (exp_of ce) = wh ∧ type_wh ns db st [] wh t
+Proof
+  strip_tac >> completeInduct_on `k` >>
+  recInduct exp_of_ind >> rw[exp_of_def]
+  >- gvs[Once type_cexp_cases]
+  >- (
+    Cases_on `p` >> gvs[op_of_def]
+    >- (
+      simp[eval_wh_to_def, type_wh_cases, SF ETA_ss] >>
+      goal_assum $ drule_at Any >> simp[]
+      )
+    >- (
+      gvs[Once type_cexp_cases]
+      >- (
+        simp[eval_wh_to_def, get_atoms_def] >>
+        simp[Once type_wh_cases] >> simp[Once type_cexp_cases]
+        ) >>
+      imp_res_tac get_PrimTys_SOME >>
+      gvs[eval_wh_to_def, MAP_MAP_o, combinTheory.o_DEF] >>
+      IF_CASES_TAC >> gvs[]
+      >- (
+        qspec_then `xs` assume_tac $ GEN_ALL get_atoms_MAP_Diverge >>
+        reverse $ Cases_on `xs` >> gvs[combinTheory.K_DEF]
+        >- simp[type_wh_cases, type_ok] >>
+        simp[get_atoms_def] >>
+        qspecl_then [`[]`,`pt`,`a`,`[]`]
+          assume_tac $ GEN_ALL eval_op_type_safe >> gvs[] >>
+        Cases_on `pt = Bool` >> gvs[]
+        >- (IF_CASES_TAC >> simp[type_wh_cases] >> simp[Once type_cexp_cases]) >>
+        simp[type_wh_cases] >> simp[Once type_cexp_cases, get_PrimTys_def] >>
+        simp[type_atom_op_cases]
+        ) >>
+      CASE_TAC >> gvs[] >- simp[type_wh_cases, type_ok] >>
+      CASE_TAC >> gvs[]
+      >- (
+        gvs[get_atoms_SOME_NONE_eq, LIST_REL_EL_EQN, EL_MAP, MEM_EL, PULL_EXISTS] >>
+        first_x_assum drule >> strip_tac >>
+        last_x_assum $ qspec_then `k - 1` mp_tac >> simp[] >>
+        disch_then drule_all >> strip_tac >>
+        qmatch_asmsub_abbrev_tac `type_wh _ _ _ _ atom` >>
+        imp_res_tac type_atom_op_no_Bool >>
+        drule type_wh_PrimTy_eq_wh_Atom >> gvs[MEM_EL] >>
+        impl_tac >- (CCONTR_TAC >> gvs[]) >> rw[] >>
+        pop_assum kall_tac >> first_x_assum $ qspec_then `n` assume_tac >> gvs[]
+        ) >>
+      gvs[get_atoms_SOME_SOME_eq] >> rename1 `MAP wh_Atom atoms` >>
+      gvs[MAP_EQ_EVERY2] >>
+      `LIST_REL type_lit atoms pts` by (
+        gvs[LIST_REL_EL_EQN, EL_MAP] >> rw[] >>
+        ntac 2 (first_x_assum drule >> strip_tac) >>
+        last_x_assum $ qspec_then `k - 1` assume_tac >> gvs[] >>
+        pop_assum drule_all >> gvs[] >> simp[Once type_wh_cases] >>
+        simp[Once type_cexp_cases, get_PrimTys_def, type_atom_op_cases]) >>
+      qspecl_then [`pts`,`pt`,`a`,`atoms`]
+        assume_tac $ GEN_ALL eval_op_type_safe >> gvs[] >>
+      Cases_on `pt = Bool` >> gvs[]
+      >- (IF_CASES_TAC >> simp[type_wh_cases, Once type_cexp_cases]) >>
+      simp[type_wh_cases] >>
+      simp[Once type_cexp_cases, get_PrimTys_def, type_atom_op_def]
+      )
+    >- (
+      pop_assum mp_tac >> simp[Once type_cexp_cases] >> rw[] >>
+      simp[eval_wh_to_def] >> reverse $ IF_CASES_TAC >> gvs[]
+      >- (FULL_CASE_TAC >> gvs[])
+      >- (
+        simp[type_wh_cases] >>
+        irule type_cexp_type_ok_unit >> simp[] >>
+        rpt $ goal_assum $ drule_at Any >> simp[]
+        ) >>
+      FULL_CASE_TAC >> gvs[] >>
+      last_x_assum $ qspec_then `k - 1` mp_tac >> simp[] >>
+      ntac 2 $ disch_then drule >>
+      disch_then $ qspecl_then [`e1`,`t1`] mp_tac >> gvs[] >>
+      simp[type_wh_cases]
+      )
+    )
+  >- (
+    gvs[eval_wh_to_def] >> rw[]
+    >- (
+      simp[type_wh_cases] >> irule type_cexp_type_ok_unit >> simp[] >>
+      rpt $ goal_assum $ drule_at Any >> simp[]
+      ) >>
+    qpat_x_assum `type_cexp _ _ _ _ _ _` mp_tac >> rw[Once type_cexp_cases] >>
+    last_x_assum $ qspec_then `k - 1` mp_tac >> simp[] >>
+    ntac 2 $ disch_then drule >>
+    disch_then $ qspecl_then [`substc1 v x y`,`t`] mp_tac >>
+    simp[subst_exp_of, FMAP_MAP2_FUPDATE] >> impl_tac
+    >- (irule type_cexp_closing_subst1 >> simp[] >> goal_assum drule >> simp[]) >>
+    simp[bind1_def] >> IF_CASES_TAC >> gvs[] >>
+    imp_res_tac type_cexp_freevars_cexp >> gvs[closed_def, freevars_exp_of]
+    )
+  >- (
+    cheat (* TODO Apps case *)
+    )
+  >- (
+    imp_res_tac type_cexp_cexp_wf >> gvs[cexp_wf_def] >>
+    Cases_on `vs` >> gvs[Lams_def] >> simp[eval_wh_to_def] >>
+    simp[Once type_wh_cases] >>
+    goal_assum drule >> simp[exp_of_def, Lams_def]
+    )
+  >- (
+    simp[eval_wh_to_def] >> rw[]
+    >- (
+      simp[type_wh_cases] >> irule type_cexp_type_ok_unit >> simp[] >>
+      rpt $ goal_assum $ drule_at Any >> simp[]
+      ) >>
+    qpat_x_assum `type_cexp _ _ _ _ _ _` mp_tac >> rw[Once type_cexp_cases] >>
+    last_x_assum $ qspec_then `k - 1` mp_tac >> simp[] >>
+    ntac 2 $ disch_then drule >>
+    disch_then $ qspecl_then
+      [`substc (FEMPTY |++ MAP (λ(g,x). (g, Letrec () rs x)) rs) x`,`t`] mp_tac >>
+    simp[subst_exp_of, FMAP_MAP2_FUPDATE_LIST] >> impl_tac
+    >- (
+      irule type_cexp_closing_subst >> simp[] >> goal_assum $ drule_at Any >>
+      imp_res_tac LIST_REL_LENGTH >> simp[MAP_REVERSE, MAP_ZIP] >>
+      simp[MAP_MAP_o, combinTheory.o_DEF, LAMBDA_PROD, GSYM FST_THM] >> rw[] >>
+      gvs[LIST_REL_EL_EQN, EL_MAP] >> rw[] >>
+      pairarg_tac >> gvs[] >> pairarg_tac >> gvs[] >>
+      simp[Once type_cexp_cases] >>
+      qexists_tac `MAP (tshift_scheme vars) schemes` >>
+      gvs[MAP_REVERSE, MAP_ZIP_ALT, MAP_MAP_o, combinTheory.o_DEF, LAMBDA_PROD] >>
+      first_assum drule >>
+      pop_assum (fn th => pop_assum (fn th' => rewrite_tac[th,th'])) >>
+      simp[] >> strip_tac >> reverse $ rw[]
+      >- (
+        gvs[EVERY_MAP, EVERY_MEM, FORALL_PROD] >> rw[] >>
+        first_x_assum drule >> rw[] >> drule type_ok_shift_db >> simp[]
+        ) >>
+      rw[LIST_REL_EL_EQN, EL_MAP] >> rename1 `EL m _` >>
+      qmatch_goalsub_abbrev_tac `_ a (_ b)` >>
+      PairCases_on `a` >> PairCases_on `b` >> gvs[] >>
+      first_x_assum drule >> rw[] >> drule type_cexp_shift_db >> simp[] >>
+      disch_then $ qspecl_then [`b0`,`vars`] mp_tac >>
+      simp[MAP_REVERSE, MAP_ZIP_ALT, MAP_MAP_o, combinTheory.o_DEF] >>
+      simp[GSYM shift_db_shift_db] >> rw[] >>
+      irule quotientTheory.EQ_IMPLIES >> goal_assum drule >>
+      rpt (AP_TERM_TAC ORELSE AP_THM_TAC) >> simp[LAMBDA_PROD]
+      ) >>
+    simp[bind_def, subst_funs_def] >>
+    simp[MAP_MAP_o, combinTheory.o_DEF, LAMBDA_PROD, exp_of_def] >>
+    IF_CASES_TAC >> gvs[] >> rename1 `false` >>
+    gvs[flookup_fupdate_list] >> every_case_tac >> gvs[] >>
+    imp_res_tac ALOOKUP_MEM >> gvs[MEM_MAP] >> pairarg_tac >> gvs[] >>
+    gvs[MAP_MAP_o, combinTheory.o_DEF, LAMBDA_PROD, GSYM FST_THM, freevars_exp_of]
+    >- (
+      gvs[MEM_EL, LIST_REL_EL_EQN] >>
+      qpat_x_assum `_ = EL _ _` $ assume_tac o GSYM >>
+      first_x_assum drule >> strip_tac >> gvs[] >> pairarg_tac >> gvs[] >>
+      imp_res_tac type_cexp_freevars_cexp >>
+      gvs[ZIP_MAP, MAP_MAP_o, combinTheory.o_DEF, LAMBDA_PROD] >>
+      gvs[pred_setTheory.SUBSET_DEF, MEM_MAP, PULL_EXISTS, EXISTS_PROD, MEM_ZIP] >>
+      metis_tac[MEM_EL]
+      )
+    >- (
+      pop_assum kall_tac >>
+      gvs[EXISTS_MAP, EXISTS_MEM] >> pairarg_tac >> gvs[freevars_exp_of] >>
+      gvs[MEM_EL, LIST_REL_EL_EQN] >>
+      qpat_x_assum `_ = EL _ _` $ assume_tac o GSYM >>
+      first_x_assum drule >> strip_tac >> gvs[] >> pairarg_tac >> gvs[] >>
+      imp_res_tac type_cexp_freevars_cexp >>
+      gvs[ZIP_MAP, MAP_MAP_o, combinTheory.o_DEF, LAMBDA_PROD] >>
+      gvs[pred_setTheory.SUBSET_DEF, MEM_MAP, PULL_EXISTS, EXISTS_PROD, MEM_ZIP] >>
+      metis_tac[MEM_EL]
+      )
+    )
+  >- (
+    cheat (* TODO Case case *)
+    )
+QED
 
 (********************)
 
